\documentclass[12pt, a4paper]{report}
\usepackage[utf8]{inputenc}
\usepackage{polski}
\usepackage{amssymb}
\usepackage{amsmath}
\usepackage{fancyhdr}
\usepackage{multicol}
\usepackage{graphicx}
\setlength{\voffset}{-0.75in}
\setlength{\headsep}{5pt}
\setlength{\hoffset}{-40pt}
\setlength{\textwidth}{500pt}
\setlength{\textheight}{770pt}
\setlength{\parindent}{0em}

\begin{document}

\begin{center}
\large{Sprawozdanie programu Burgers Equation 2024}
\end{center}

$u_{i,j}=u(x_{i},t_{j})=u(i\cdot h,j\cdot k)$\\
$h=0.1, k=0.005$\\
Warunek początkowy: $u_{0,j}=u_{M-1,j}=0\\
\hspace*{4.1cm} u_{i,0}=e^{-(x_{i}-x_{mid})^{2}}$

\begin{center}
\large{Równania}
\end{center}
\begin{enumerate}
\item $\frac{\partial u}{\partial t}+\frac{\partial u}{\partial x}=0$
\item $\frac{\partial u}{\partial t}+u\frac{\partial u}{\partial x}=0$
\item $\frac{\partial u}{\partial t}-\beta\frac{\partial^{2} u}{\partial x^{2}}=0$
\item $\frac{\partial u}{\partial t}+u\frac{\partial u}{\partial x}-\beta\frac{\partial^{2} u}{\partial x^{2}}=0$ (Równanie Burgers'a)
\end{enumerate}

\begin{center}
\large{Metoda Eulera}
\end{center}

\begin{enumerate}
\item$\frac{1}{k}(u_{i,j+1}-u_{i,j})+\frac{1}{2h}(u_{i+1,j}-u_{i-1,j})=0$\\\\
$u_{i,j+1}=u_{i,j}-\frac{k}{2h}(u_{i+1,j}-u_{i-1,j})$

\item$\frac{1}{k}(u_{i,j+1}-u_{i,j})+\frac{1}{4h}(u_{i+1,j}^{2}-u_{i-1,j}^{2})=0$\\\\
$u_{i,j+1}=u_{i,j}-\frac{k}{4h}(u_{i+1,j}^{2}-u_{i-1,j}^{2})$

\item$\frac{1}{k}(u_{i,j+1}-u_{i,j})-\frac{\beta}{h^{2}}(u_{i+1,j}-2u_{i,j}+u_{i-1,j})=0$\\\\
$u_{i,j+1}=u_{i,j}+\frac{\beta k}{h^{2}}(u_{i+1,j}-2u_{i,j}+u_{i-1,j})$

\item$\frac{1}{k}(u_{i,j+1}-u_{i,j})+\frac{1}{4h}(u_{i+1,j}^{2}-u_{i-1,j}^{2})-\frac{\beta}{h^{2}}(u_{i+1,j}-2u_{i,j}+u_{i-1,j})=0$\\\\
$u_{i,j+1}=u_{i,j}-\frac{k}{4h}(u_{i+1,j}^{2}-u_{i-1,j}^{2})+\frac{\beta k}{h^{2}}(u_{i+1,j}-2u_{i,j}+u_{i-1,j})$
\end{enumerate}

\begin{center}
\large{Metoda Rungego-Kutty 2-go rzędu}
\end{center}

\begin{enumerate}
\item$v_{i,j+1}=u_{i,j}-\frac{k}{4h}(u_{i+1,j}-u_{i-1,j})$\\\\
$u_{i,j+1}=u_{i,j}-\frac{k}{2h}(v_{i+1,j+1}-v_{i-1,j+1})$

\item$v_{i,j+1}=u_{i,j}-\frac{k}{8h}(u_{i+1,j}^{2}-u_{i-1,j}^{2})$\\\\
$u_{i,j+1}=u_{i,j}-\frac{k}{4h}(v_{i+1,j+1}^{2}-v_{i-1,j+1}^{2})$

\item$v_{i,j+1}=u_{i,j}+\frac{\beta k}{2h^{2}}(u_{i+1,j}-2u_{i,j}+u_{i-1,j})$\\\\
$u_{i,j+1}=u_{i,j}+\frac{\beta k}{h^{2}}(v_{i+1,j+1}-2v_{i,j+1}+v_{i-1,j+1})$

\item$v_{i,j+1}=u_{i,j}-\frac{k}{8h}(u_{i+1,j}^{2}-u_{i-1,j}^{2})+\frac{\beta k}{2h^{2}}(u_{i+1,j}-2u_{i,j}+u_{i-1,j})$\\\\
$u_{i,j+1}=u_{i,j}-\frac{k}{4h}(v_{i+1,j+1}^{2}-v_{i-1,j+1}^{2})+\frac{\beta k}{h^{2}}(v_{i+1,j+1}-2v_{i,j+1}+v_{i-1,j+1})$
\end{enumerate}

\newpage

\begin{center}
\large{Metoda Niejawna}
\end{center}

\begin{enumerate}
 \setcounter{enumi}{2}

\item$\frac{1}{k}(u_{i,j}-u_{i,j-1})-\frac{\beta}{h^{2}}(u_{i+1,j}-2u_{i,j}+u_{i-1,j})=0$\\\\
$u_{i,j-1}=-\frac{\beta k}{h^{2}}u_{i-1,j}+(1+2\frac{\beta k}{h^{2}})u_{i,j}-\frac{\beta k}{h^{2}}u_{i+1,j}$\\\\
$A=
\begin{bmatrix}
1+2s & -s & 0 & \cdots & 0\\
-s & 1+2s & -s & \cdots & 0\\
0 & -s & 1+2s & \cdots & 0\\
\cdots & \cdots & \cdots & \cdots & \cdots\\
0 & 0 & 0 & \cdots & 1+2s\\
\end{bmatrix}$
$,s=\frac{\beta k}{h^{2}}$\\\\
$u_{i,j}=A^{-1}u_{j-1}$

\item$\frac{1}{k}(u_{i,j}-u_{i,j-1})+\frac{1}{4h}(u_{i+1,j-1}^{2}-u_{i-1,j-1}^{2})-\frac{\beta}{h^{2}}(u_{i+1,j}-2u_{i,j}+u_{i-1,j})=0$\\\\
$u_{i,j-1}-\frac{k}{4h}(u_{i+1,j-1}^{2}-u_{i-1,j-1}^{2})=-\frac{\beta k}{h^{2}}u_{i-1,j}+(1+2\frac{\beta k}{h^{2}})u_{i,j}-\frac{\beta k}{h^{2}}u_{i+1,j}$\\\\
$A=
\begin{bmatrix}
1+2s & -s & 0 & \cdots & 0\\
-s & 1+2s & -s & \cdots & 0\\
0 & -s & 1+2s & \cdots & 0\\
\cdots & \cdots & \cdots & \cdots & \cdots\\
0 & 0 & 0 & \cdots & 1+2s\\
\end{bmatrix}$
$,s=\frac{\beta k}{h^{2}}$\\\\
$u_{i,j}=A^{-1}(u_{i,j-1}-\frac{k}{4h}(u_{i+1,j-1}^{2}-u_{i-1,j-1}^{2}))$
\end{enumerate}

\end{document}